{
  "@context": {
    "dct": "http://purl.org/dc/terms/",
    "owl": "http://www.w3.org/2002/07/owl#",
    "rdf": "http://www.w3.org/1999/02/22-rdf-syntax-ns#",
    "rdfa": "http://www.w3.org/ns/rdfa#",
    "rdfs": "http://www.w3.org/2000/01/rdf-schema#",
    "schema": "http://schema.org/",
    "xsd": "http://www.w3.org/2001/XMLSchema#",
    "sbm": "http://schema.saltbaymedia.com/ontology/v1/"
  },
  "@graph": [
    {
      "@id": "sbm:CreativeWorkRelationship",
      "@type": "rdfs:Class",
      "rdfs:comment": "Qualifies how one CreativeWork is related to another CreativeWork. Since this is the value-add, classify it as a schema:Product. In this way, we can use schema:additionalProperty to describe the value-add.",
      "rdfs:label": "CreativeWorkRelationship",
      "rdfs:subClassOf": [{ "@id": "schema:Product"},{"@id": "schema:CreativeWork"}]
    },
    {
      "@id": "sbm:remakeOf",
      "@type": "rdf:Property",
      "rdfs:comment": "Specifies that this CreativeWork is a remake of a previously existing CreativeWork.",
      "rdfs:label": "remakeOf",
      "rdfs:subPropertyOf": { "@id": "schema:isBasedOn"},
      "schema:domainIncludes": { "@id": "schema:CreativeWork" },
      "schema:rangeIncludes": { "@id": "schema:CreativeWork" }
    },
    {
      "@id": "sbm:relatedWork",
      "@type": "rdf:Property",
      "rdfs:comment": "Specifies that this CreativeWork related to another CreativeWork through a CreativeWorkRelationship.",
      "rdfs:label": "relatedWork",
      "rdfs:subPropertyOf": { "@id": "schema:subjectOf"},
      "schema:domainIncludes": { "@id": "schema:CreativeWork" },
      "schema:rangeIncludes": { "@id": "schema:CreativeWorkRelationship" }
    },
    {
      "@id": "sbm:editor",
      "@type": "rdf:Property",
      "rdfs:comment": "Specifies a Person or Organization that edited a CreativeWork.",
      "rdfs:label": "editor",
      "rdfs:subPropertyOf": { "@id": "schema:subjectOf"},
      "schema:domainIncludes": { "@id": "schema:CreativeWork" },
      "schema:rangeIncludes": [
        { "@id": "schema:Person" },
        { "@id": "schema:Organization" }
      ]
    },
    {
      "@id": "sbm:cinematographer",
      "@type": "rdf:Property",
      "rdfs:comment": "Specifies a Person that acted as the cinematographer on a CreativeWork.",
      "rdfs:label": "cinematographer",
      "rdfs:subPropertyOf": { "@id": "schema:subjectOf"},
      "schema:domainIncludes": [
        { "@id": "schema:Clip" },
        { "@id": "schema:CreativeWorkSeason" },
        { "@id": "schema:Episode" },
        { "@id": "schema:Movie" },
        { "@id": "schema:MovieSeries" },
        { "@id": "schema:TVSeries" }
      ]
      "schema:rangeIncludes": { "@id": "schema:Person" }
    }
  ]
}
