# baseURI: http://schema.saltbaymedia.com/ontology/v1/
# imports: http://schema.org/
# prefix: sbm

@prefix : <http://schema.saltbaymedia.com/ontology/v1/> .
@prefix schema: <http://schema.org/> .
@prefix owl: <http://www.w3.org/2002/07/owl#> .
@prefix rdf: <http://www.w3.org/1999/02/22-rdf-syntax-ns#> .
@prefix rdfs: <http://www.w3.org/2000/01/rdf-schema#> .
@prefix xsd: <http://www.w3.org/2001/XMLSchema#> .
@prefix dc: <http://purl.org/dc/elements/1.1/> .
@prefix dct: <http://purl.org/dc/terms/> .
@prefix prov: <http://www.w3.org/ns/prov#> .
@prefix skos: <http://www.w3.org/2004/02/skos/core#> .

#### Ontology

<http://schema.saltbaymedia.com/ontology/v1/> a owl:Ontology ;
    rdfs:label "Salt Bay Media Ontology"@en-US ;
    rdfs:comment "An ontology for describing movies and the connections between them"@en-US ;
    dc:creator "Adam Shepherd" ; 
    dct:publisher <http://www.saltbaymedia.com/author/adam-shepherd> ;
    dc:publisher "Salt Bay Media" ;
    dct:publisher <http://www.saltbaymedia.com> ;
    dct:issued "2019-01-01"^^xsd:date ;
    dct:source "https://github.com/SaltBayMedia/Ontology"^^xsd:anyURI ;
    owl:imports <http://schema.org/> ;
    owl:versionInfo "0.1.0" .


#### Annotation Properties 

dc:creator a owl:AnnotationProperty .
dct:creator a owl:AnnotationProperty .
dc:publisher a owl:AnnotationProperty .
dct:publisher a owl:AnnotationProperty .
dct:issued a owl:AnnotationProperty .
dct:source a owl:AnnotationProperty .


#### Classes
sbm:CreativeWorkRelationship a owl:Class ;
    rdfs:label "CreativeWorkRelationship"@en-us ;
    rdfs:comment """Qualifies how one CreativeWork is related to another CreativeWork. 
        Since this is the value-add, classify it as a schema:Product.
        In this way, we can use schema:additionalProperty to describe the value-add."""@en-us ;
    rdfs:subClassOf schema:Product, schema:CreativeWork ;
    rdfs:subClassOf [ a owl:Restriction ;
            owl:minCardinality "1"^^xsd:nonNegativeInteger ;
            owl:onProperty schema:category ] .

sbm:Agent a owl:Class ;
    dfs:label "CreativeWorkRelationship"@en-us ;
    rdfs:comment """A superclass for classifying entities act in a certain role on or for a CreativeWork."""@en-us ;
    rdfs:subClassOf CreativeWorkEditorRangeRestriction ;

#### Object Properties

sbm:remakeOf a owl:ObjectProperty ;
    rdfs:label "remakeOf"@en-us ;
    rdfs:comment "Specifies that this CreativeWork is a remake of a previously existing CreativeWork."@en-us ;
    rdfs:domain schema:CreativeWork ;
    rdfs:range schema:CreativeWork ;
    rdfs:subPropertyOf schema:isBasedOn .

sbm:relatedWork a owl:ObjectProperty ;
    rdfs:label "relatedWork"@en-us ;
    rdfs:comment "Specifies that this CreativeWork related to another CreativeWork through a CreativeWorkRelationship."@en-us ;
    rdfs:domain schema:CreativeWork ;
    rdfs:range schema:CreativeWorkRelationship ;
    rdfs:subPropertyOf schema:subjectOf .

sbm:editor a owl:ObjectProperty ;
    rdfs:label "editor"@en-us ;
    rdfs:comment "Specifies a Person or Organization that edited a CreativeWork."@en-us ;
    rdfs:domain schema:CreativeWork ;
    rdfs:range sbm:Agent ;
    rdfs:subPropertyOf schema:subjectOf .

sbm:cinematographer a owl:ObjectProperty ;
    rdfs:label "editor"@en-us ;
    rdfs:comment "Specifies a Person that acted as the cinematographer on a CreativeWork."@en-us ;
    rdfs:domain schema:CreativeWork ;
    rdfs:range sbm:Person ;
    rdfs:subPropertyOf schema:subjectOf .


#### Axioms ####

schema:Person rdfs:subClassOf sbm:Agent ;
schema:Organization rdfs:subClassOf sbm:Agent ;
    
sbm:CreativeWorkEditorRangeRestriction a owl:Restriction ;
    owl:onProperty sbm:editor ;
    owl:oneOf schema:Person, schema:Organization .

